Strata/Languages/Core/WF.lean
@@ -138,15 +138,16 @@ structure WFAxiomDeclarationProp (p : Program) (f : Axiom) : Prop where
 structure WFDistinctDeclarationProp (p : Program) (l : Expression.Ident) (es : List (Expression.Expr)) : Prop where
 
 structure WFProcedureProp (p : Program) (d : Procedure) : Prop where
-  wfstmts : WFStatementsProp p d.body.stmts
-  wfloclnd : (HasVarsImp.definedVars (P:=Expression) d.body.stmts).Nodup
+  bodyIsStructured : ∃ ss, d.body = .structured ss
+  wfstmts : ∀ ss, d.body = .structured ss → WFStatementsProp p ss
+  wfloclnd : ∀ ss, d.body = .structured ss → (HasVarsImp.definedVars (P:=Expression) ss).Nodup
   inputsNodup : (ListMap.keys d.header.inputs).Nodup
   outputsNodup : (ListMap.keys d.header.outputs).Nodup
   ioNotOld : ∀ id ∈ ListMap.keys d.header.inputs ++ ListMap.keys d.header.outputs,
       ∀ x, id ≠ CoreIdent.mkOld x
   wfspec : WFSpecProp p d.spec d
-  -- There is no exit statement that cannot be caught by any block in the procedure.
-  bodyExitsCovered : Stmt.exitsCoveredByBlocks.Block.exitsCoveredByBlocks [] d.body.stmts
+  bodyExitsCovered : ∀ ss, d.body = .structured ss →
+    Stmt.exitsCoveredByBlocks.Block.exitsCoveredByBlocks [] ss
 structure WFFunctionProp (p : Program) (f : Function) : Prop where
 
 structure WFRecFuncBlockProp (p : Program) (fs : List Function) : Prop where
